more examples

src/examples/GPU.Reduction.fst
@@ -12,6 +12,8 @@ open Pulse.Lib.BigStar
 open GPU
 open GPU.Scalars
 open GPU.Barrier.RPM
+open FStar.Seq
+module GA = GPU.Array
 
 module A = Pulse.Lib.Array
 module SZ = FStar.SizeT
@@ -19,488 +21,121 @@ module U32 = FStar.UInt32
 
 let size : SZ.t = 1024sz
 
-let rec log2 (n: nat{n <> 0}): GTot (r:nat{r < n}) =
-  if n = 1 then 0 else 1 + log2 (n / 2)
-let rec pow_log_lemma (n: nat) : Lemma (log2 (pow2 n) = n) =
-  if n = 0 then () else pow_log_lemma (n - 1)
-
-[@@ CPrologue "__device__"]
-let spow2 (s : SZ.t{s < 32}) : r:SZ.t{SZ.v r == pow2 (SZ.v s)} =
-  let r = SZ.uint32_to_sizet (U32.shift_left 1ul (sizet_to_u32 s)) in
-  assume (SZ.v r == pow2 (SZ.v s)); // prove this from UInt library
-  r
-
-let div_pow2 (i tid: nat) : GTot bool =
-  (=) #int (tid % pow2 i) 0
-
-[@@ CPrologue "__device__"]
-let sdiv_pow2 (i:SZ.t{i < 32}) (tid: SZ.t): bool =
-  SZ.rem tid (spow2 i) = 0sz
-
-let rec div_pow2_lemma (i j tid: nat):
-  Lemma
-    (requires i < j)
-    (ensures (div_pow2 j tid) ==> (div_pow2 i tid))
-  = if not (div_pow2 j tid) then () else (
-      if i = j - 1 then () else div_pow2_lemma i (j - 1) tid;
-      FStar.Math.Lemmas.mod_mult_exact tid (pow2 (j - 1)) 2
-  )
-
-let min (a b: nat) : GTot nat =
-  if a < b then a else b
-
-[@@ CPrologue "__device__"]
-let smin (a b: SZ.t): SZ.t = if a <^ b then a else b
-
-// Pure SUM
-
-let rec sum_seq (s: Seq.seq U64.t) (i j : nat)
-  : Ghost U64.t (requires i < j /\ j <= Seq.length s)
-                (ensures fun _ -> True)
-                (decreases j - i)
-=
-  if i = j - 1 then Seq.index s i else U64.add_mod (Seq.index s i) (sum_seq s (i + 1) j)
-
-let add_mod_assoc (a b c: U64.t): Lemma (U64.add_mod (U64.add_mod a b) c = U64.add_mod a (U64.add_mod b c)) = admit()
-
-let rec sum_seq_lemma (s: Seq.seq U64.t) (i j k:nat):
-  Lemma (requires i < j && j < k && k <= Seq.length s)
-        (ensures sum_seq s i k = U64.add_mod (sum_seq s i j) (sum_seq s j k)) (decreases j - i) =
-    if i = j - 1 then () else (sum_seq_lemma s (i + 1) j k; add_mod_assoc (Seq.index s i) (sum_seq s (i + 1) j) (sum_seq s j k))
-
-// Impure SUM
-
-let gpu_pts_to_slice_sum_inner
-  (#sz:nat)
-  (r: gpu_array U64.t sz)
-  (i j:nat)
-  (v: Seq.seq U64.t)
-  (s: Seq.seq U64.t)
-: slprop = gpu_pts_to_array_slice r i j s ** pure (i < j /\ j <= sz /\ Seq.length v = sz /\ Seq.length s = j - i /\ Seq.index s 0 = sum_seq v i j)
-
-let gpu_pts_to_slice_sum
-  (#sz:nat)
-  (r: gpu_array U64.t sz)
-  (i j:nat)
-  (v: Seq.seq U64.t)
-: slprop = if_ (i < j && j <= sz) (exists* s. gpu_pts_to_slice_sum_inner #sz r i j v s)
-
-// Barrier
-
-let barrier_matrix (nth: nat) (r : gpu_array U64.t nth) (v: Seq.seq U64.t) (it from to: nat): slprop =
-  if_ (from = to + pow2 it)
-      (if_ (not (div_pow2 (it + 1) from) && (div_pow2 it from))
-           (gpu_pts_to_slice_sum r from (min (from + pow2 it) nth) v))
-
-// #push-options "--debug SMTFail --split_queries always"
-// #push-options "--print_implicits"
-
-
-ghost fn unfold_barrier_matrix (nth: nat) (r : gpu_array U64.t nth) (v: erased (Seq.seq U64.t))
- (it from to: nat)
-  requires barrier_matrix nth r v it from to
-  ensures  if_ (op_Equality #int from (to + pow2 it)) (if_ (not (div_pow2 (it + 1) from) && (div_pow2 it from)) (gpu_pts_to_slice_sum r from (min (from + pow2 it) nth) v))
+(* Reduces a simple scalar array with the addition operation, leaving
+the result in the 0th index of the original array (overwriting that element). *)
+[@@CPrologue "__device__"]
+fn k_reduce
+  (#tt : Type0)
+  {| d : simple_scalar tt |}
+  (size : SZ.t)
+  (a : gpu_array tt size)
+  (#v : erased (seq tt))
+  requires gpu ** GA.gpu_pts_to_array a v ** pure (size > 0)
+  returns  r : tt
+  ensures  gpu ** GA.gpu_pts_to_array a v
 {
-  unfold (barrier_matrix nth r v it from to)
-}
+  let mut i = 0sz;
+  let mut r : tt = zero #tt #d;
+  unfold (gpu_pts_to_array a v);
 
-// let even n : prop = n % 2 == 0
-// let odd  n : prop = ~ (n % 2 == 0)
-
-// let div_helper (n : nat) :
-//   Lemma ((~(even (n+1))) <==>  even n) = ()
-
-val lemma_div_exact: a:int -> p:pos -> Lemma
-  (a % p = 0 <==> a = p * (a / p))
-let lemma_div_exact a p = ()
-
-let div_pow2_lemma_2 (it tid: nat):
-  Lemma (
-    (not (div_pow2 (it + 1) (tid + pow2 it)) && div_pow2 it (tid + pow2 it))
-    <==>
-    div_pow2 (it + 1) tid
-  ) =
-    calc (<==>) {
-      (not (div_pow2 (it + 1) (tid + pow2 it))) && div_pow2 it (tid + pow2 it) <: prop;
-      <==> {}
-      (tid + pow2 it)                       % (2 * pow2 it) <> 0 && (tid + pow2 it) % pow2 it = 0 <: prop;
-      <==> { FStar.Math.Lemmas.lemma_div_mod_plus tid 1 (pow2 it) }
-      (tid + pow2 it)                       % (2 * pow2 it) <> 0 && tid % pow2 it = 0 <: prop;
-      <==> { lemma_div_exact tid (pow2 it) }
-      (pow2 it * (tid / pow2 it) + pow2 it) % (2 * pow2 it) <> 0 && tid % pow2 it = 0 <: prop;
-      <==> { FStar.Math.Lemmas.distributivity_add_right (pow2 it) (tid / pow2 it) 1 }
-      (pow2 it * (tid / pow2 it + 1))       % (2 * pow2 it) <> 0 && tid % pow2 it = 0 <: prop;
-      <==> { FStar.Math.Lemmas.modulo_scale_lemma (tid / pow2 it + 1) (pow2 it) 2 }
-      pow2 it * ((tid / pow2 it + 1) % 2)                   <> 0 && tid % pow2 it = 0 <: prop;
-      <==> {}
-      pow2 it * ((tid / pow2 it) % 2)                        = 0 && tid % pow2 it = 0 <: prop;
-      <==> { FStar.Math.Lemmas.modulo_scale_lemma (tid / pow2 it) (pow2 it) 2 }
-      (pow2 it * (tid / pow2 it)) % (2 * pow2 it)            = 0 && tid % pow2 it = 0 <: prop;
-      <==> { lemma_div_exact tid (pow2 it) }
-      tid % (2 * pow2 it)                                    = 0 && tid % pow2 it = 0 <: prop;
-      <==> { div_pow2_lemma it (it + 1) tid }
-      div_pow2 (it + 1) tid;
-    }
-
-ghost fn fold_barrier_matrix_true
-  (nth : nat)
-  (r: gpu_array U64.t nth)
-  (v: Seq.seq U64.t { Seq.length v == nth })
-  (it: nat)
-  (tid: nat { tid <= nth /\ tid >= pow2 it })
-  (to: nat)
-  requires if_ (op_Equality #int to (tid - pow2 it))
-             (if_ (not (div_pow2 (it + 1) tid) && div_pow2 it tid)
-               (gpu_pts_to_slice_sum r tid (min (tid + pow2 it) nth) v))
-  ensures  barrier_matrix nth r v it tid to
-{
-  fold (barrier_matrix nth r v it tid to);
-}
-
-ghost fn fold_barrier_matrix_false
-  (nth : nat)
-  (r: gpu_array U64.t nth)
-  (v: Seq.seq U64.t { Seq.length v == nth })
-  (it: nat)
-  (tid: nat { tid <= nth /\ tid < pow2 it })
-  (to: nat { to <= nth })
-  requires emp
-  ensures  barrier_matrix nth r v it tid to
-{
-  assert (pure (tid < to + pow2 it /\ not (op_Equality #int tid (to + pow2 it))));
-  if_intro_false (if_ (not (div_pow2 (it + 1) tid) && (div_pow2 it tid)) (gpu_pts_to_slice_sum r tid (min (tid + pow2 it) nth) v));
-  // (op_Equality #int tid (to + pow2 it))
-  fold (barrier_matrix nth r v it tid to);
-}
-
-// #push-options "--print_implicits --print_bound_var_types"
-
-ghost
-fn mk_barrier_pre
-  (nth : SZ.t { 0 < SZ.v nth /\ SZ.v nth <= 1024 })
-  (r : gpu_array U64.t nth)
-  (vv: erased (Seq.seq U64.t))
-  (#_: squash (Seq.length vv == nth))
-  (tid : SZ.t{SZ.v tid < nth})
-  (it: SZ.t{it < 31})
-  requires if_ (not (div_pow2 (it + 1) tid) && div_pow2 it tid)
-      (gpu_pts_to_slice_sum #nth r tid (min (tid + pow2 it) nth) vv)
-  ensures bigstar 0 nth (barrier_matrix nth r vv it tid)
-{
-  open FStar.SizeT;
-  if (tid >=^ spow2 it) {
-    bigstar_if_intro 0 nth (tid - pow2 it) (fun _ -> if_ (not (div_pow2 (it + 1) tid) && (div_pow2 it tid)) (gpu_pts_to_slice_sum r tid (min (tid + pow2 it) nth) vv));
-    bigstar_map #_ #_ #0 #nth #(fun (i:nat { 0 <= i /\ i < nth }) -> _ i) (fold_barrier_matrix_true nth r vv it tid);
-  } else {
-    FStar.Math.Lemmas.modulo_lemma tid (spow2 it);
-    FStar.Math.Lemmas.modulo_lemma 0 (spow2 (it +^ 1sz));
-    // assert (pure ((tid <: nat) <> 0 ==> not (div_pow2 it tid)));
-    // assert (pure ((tid <: nat) = 0 ==> (div_pow2 (it + 1) tid)));
-    if_rewrite_bool (op_Negation (div_pow2 (SZ.v it + 1) (SZ.v tid)) && div_pow2 (SZ.v it) (SZ.v tid)) false _;
-    if_elim_false _;
-
-    bigstar_emp_intro 0 nth;
-    bigstar_map #_ #_ #0 #nth #(fun (i:nat { 0 <= i /\ i < nth }) -> emp) (fold_barrier_matrix_false nth r vv it tid);
-  }
-}
-
-#set-options "--print_implicits"
-
-[@@ CPrologue "__device__"]
-fn iteration
-  (nth : SZ.t { 0 < SZ.v nth /\ SZ.v nth <= 1024 })
-  (r : gpu_array U64.t nth)
-  (vv: erased (Seq.seq U64.t))
-  (#_: squash (Seq.length vv == nth))
-  (tid : SZ.t{SZ.v tid < nth})
-  (it: SZ.t{it < 31})
-  requires gpu
-    ** mbarrier_tok nth (barrier_matrix nth r vv) it tid
-    ** if_ (div_pow2 it tid) (gpu_pts_to_slice_sum r tid (min (tid + pow2 it) nth) vv)
-  ensures gpu
-    ** mbarrier_tok nth (barrier_matrix nth r vv) (it+1) tid
-    ** if_ (div_pow2 (it+1) tid) (gpu_pts_to_slice_sum r tid (min (tid + pow2 (it + 1)) nth) vv)
-{
-  open FStar.SizeT;
-  assume_ (pure (forall (x:nat). FStar.SizeT.fits x)); // CHEATING overflow
-  assert (pure (Seq.length vv = nth));
-
-  case_split (div_pow2 (it + 1) tid) (if_ (div_pow2 it tid) (gpu_pts_to_slice_sum r tid (min (tid + pow2 it) nth) vv));
-  if_flatten #(div_pow2 (it + 1) tid);
-  if_flatten #(not (div_pow2 (it + 1) tid));
-  
-  div_pow2_lemma it (it + 1) tid;
-  rewrite (if_ (div_pow2 (it + 1) tid && div_pow2 it tid)
-            (gpu_pts_to_slice_sum r tid (min (tid + pow2 it) nth) vv))
-      as (if_ (div_pow2 (it + 1) tid)
-            (gpu_pts_to_slice_sum r tid (min (tid + pow2 it) nth) vv));
-
-  mk_barrier_pre nth r vv tid it;
-  mbarrier_wait #(SZ.v nth) #(barrier_matrix nth r vv) #(SZ.v it) #(SZ.v tid);
-
-  bigstar_map #_ #_ #0 #nth (fun (from: nat { 0 <= from /\ from < nth }) -> unfold_barrier_matrix nth r vv it from tid);
-
-  // combine (div_pow2 (it + 1) tid) (gpu_pts_to_slice_sum r tid (min (tid + pow2 it) nth) vv) _;
-
-  let middle : SZ.t = smin (tid +^ spow2 it) nth;
-  (* We do not use end_ in extracted code, so we can use a nat and erase it
-  so there are no traces in the extracted C. *)
-  let end_   : erased nat = hide (min (tid + 2 * pow2 it) nth);
-
-  if (tid +^ spow2 it <^ nth) {
-    bigstar_if_elim #_ #0
-      #nth (tid + pow2 it)
-      (fun (from: nat) -> if_ (not (div_pow2 (it + 1) from) && (div_pow2 it from)) (gpu_pts_to_slice_sum r from (min (from + pow2 it) nth) vv));
-
-    let b = sdiv_pow2 (it +^ 1sz) tid;
-    
-    assume_ (pure (b <==> (div_pow2 (SZ.v it + 1) (SZ.v tid))));
-    rewrite each (div_pow2 (SZ.v it + 1) (SZ.v tid)) as b;
-
-    div_pow2_lemma_2 it tid;
-    combine
-      b
-      (gpu_pts_to_slice_sum r (tid + pow2 it) (min (tid + pow2 it + pow2 it) nth) vv)
-      _;
-      
-    if b {
-      assert (pure (div_pow2 (SZ.v it + 1) (SZ.v tid)));
-      if_elim_true _;
-
-      unfold (gpu_pts_to_slice_sum r tid middle vv);
-      if_elim_true (exists* s. gpu_pts_to_slice_sum_inner r tid middle vv s);
-      unfold gpu_pts_to_slice_sum_inner;
-      unfold (gpu_pts_to_slice_sum r middle end_ vv);
-      if_elim_true (exists* s. gpu_pts_to_slice_sum_inner r middle end_ vv s);
-      unfold gpu_pts_to_slice_sum_inner;
-
-      let s1 = gpu_array_read #U64.t #(SZ.v nth) #(SZ.v tid) #(SZ.v middle) r tid;
-      // assert (pure (s1 == sum_seq vv tid middle));
-      let s2 = gpu_array_read #U64.t #(SZ.v nth) #(SZ.v middle) #end_ r middle;
-      // assert (pure (s2 == sum_seq vv middle end_));
-      let s = U64.add_mod s1 s2;
-      sum_seq_lemma vv tid middle end_;
-      // assert (pure ( s == sum_seq vv tid end_ ));
-      gpu_array_write #U64.t #(SZ.v nth) #(SZ.v tid) #(SZ.v middle) r tid s;
-
-      gpu_slice_concat #U64.t #(SZ.v nth) r tid middle end_;
-      with seq. assert (gpu_pts_to_array_slice r tid end_ seq);
-      // assert (pure (Seq.index seq 0 == s));
-      fold (gpu_pts_to_slice_sum_inner #nth r tid end_ vv seq);
-      if_intro_true (exists* s. gpu_pts_to_slice_sum_inner #nth r tid end_ vv s);
-      fold (gpu_pts_to_slice_sum r tid end_ vv);
-      if_intro_true (gpu_pts_to_slice_sum r tid end_ vv);
-    } else {
-      if_elim_false _;
-      if_intro_false (gpu_pts_to_slice_sum r tid end_ vv);
-    }
-  } else {
-    bigstar_map #_ #_ #0 #nth #(fun (from:nat { 0 <= from /\ from < nth }) -> _ from)
-      (fun (from: nat{0 <= from /\ from < nth}) ->
-        if_rewrite_bool (op_Equality #int from (tid + pow2 it)) false _);
-    bigstar_map #_ #_ #0 #nth #(fun (from:nat { 0 <= from /\ from < nth }) -> _ from)
-      (fun (from: nat{0 <= from /\ from < nth}) ->
-        if_elim_false (if_ (not (div_pow2 (it + 1) from) && (div_pow2 it from)) (gpu_pts_to_slice_sum r from (min (from + pow2 it) nth) vv)));
-    bigstar_emp_elim #_;
-  }
-}
-
-let kpre (nth: nat) (ga1 ga2 r : gpu_array U64.t nth) (#s1 #s2: erased (Seq.seq U64.t))
-  (#_: squash ( Seq.length s1 == nth /\ Seq.length s2 == nth )) (tid:nat{tid < nth})
-  : slprop =
-    (gpu_pts_to_array #U64.t #nth ga1 #(1.0R /. Real.of_int nth) s1 **
-    gpu_pts_to_array #U64.t #nth ga2 #(1.0R /. Real.of_int nth) s2) **
-    gpu_pts_to_array1 r tid
-
-let kpost (nth: nat) (ga1 ga2 r : gpu_array U64.t nth) (#s1 #s2: erased (Seq.seq U64.t))
-  (#_: squash ( Seq.length s1 == nth /\ Seq.length s2 == nth )) (tid:nat{tid < nth})
-  : slprop =
-    ((gpu_pts_to_array #U64.t #nth ga1 #(1.0R /. Real.of_int nth) s1 **
-    gpu_pts_to_array #U64.t #nth ga2 #(1.0R /. Real.of_int nth) s2) **
-    if_ (tid = 0) (gpu_pts_to_slice_sum r 0 nth (mul s1 s2)))
-
-// #set-options "--ext pulse:env_on_err=1"
-
-[@@ CPrologue "__global__"]
-fn kernel
-  (nth : SZ.t { 0 < SZ.v nth /\ SZ.v nth <= 1024 })
-  (ga1 ga2 : gpu_array U64.t nth)
-  (r : gpu_array U64.t nth)
-  (#s1 #s2: erased (Seq.seq U64.t))
-  (#_: squash ( Seq.length s1 == nth /\ Seq.length s2 == nth ))
-  (etid : erased tid_t { (gdim_x etid <: nat) == 1ul /\ (bdim_x etid <: nat) == SZ.sizet_to_uint32 nth })
-  requires gpu ** thread_id etid ** mbarrier_tok nth (barrier_matrix nth r (mul s1 s2)) 0 (tidx_x etid) ** kpre  nth ga1 ga2 r #s1 #s2 (thread_index etid)
-  ensures  gpu ** thread_id etid ** (exists* it. mbarrier_tok nth (barrier_matrix nth r (mul s1 s2)) it (tidx_x etid)) ** kpost nth ga1 ga2 r #s1 #s2 (thread_index etid)
-{
-  let tid : U32.t = thread_idx_x ();
-  let tid : SZ.t = SZ.uint32_to_sizet tid;
-  (**)unfold (kpre nth ga1 ga2 r #s1 #s2 tid);
-
-  (**)unfold (gpu_pts_to_array #U64.t #(SZ.v nth) ga1 #(1.0R /. Real.of_int nth) s1);
-  let v1 = gpu_array_read #U64.t #(SZ.v nth) #0 #(SZ.v nth) ga1 tid #s1;
-  (**)fold (gpu_pts_to_array #U64.t #nth ga1 #(1.0R /. Real.of_int nth) s1);
-
-  (**)unfold (gpu_pts_to_array #U64.t #nth ga2 #(1.0R /. Real.of_int nth) s2);
-  let v2 = gpu_array_read #U64.t #(SZ.v nth) #0 #(SZ.v nth) ga2 tid #s2;
-  (**)fold (gpu_pts_to_array #U64.t #nth ga2 #(1.0R /. Real.of_int nth) s2);
-  
-  let vm = U64.mul_mod v1 v2;
-  let dot_v = hide (mul s1 s2);
-  
-  (**)unfold (gpu_pts_to_array1 r tid);
-  gpu_array_write #U64.t #(SZ.v nth) #(SZ.v tid) #(hide (SZ.v tid+1)) r tid vm;
-  
-  (* Reduction *)
-  let mut n = 0sz;
-
-  (**)with s. assert (gpu_pts_to_array_slice r tid (tid+1) s);
-  (**)fold (gpu_pts_to_slice_sum_inner #nth r tid (tid+1) dot_v s);
-  (**)if_intro_true (exists* s. gpu_pts_to_slice_sum_inner #nth r tid (tid + pow2 0) dot_v s);
-  (**)fold (gpu_pts_to_slice_sum r tid (tid + pow2 0) dot_v);
-  (**)if_intro_true (gpu_pts_to_slice_sum r tid (tid + pow2 0) dot_v);
-
-  while (let it = !n; (spow2 it <^ nth))
-    invariant c.
-    exists* (it:SZ.t).
-      gpu **
-      pts_to n it **
-      mbarrier_tok nth (barrier_matrix nth r dot_v) it tid **
-      if_ (div_pow2 (SZ.v it) (SZ.v tid)) (gpu_pts_to_slice_sum r tid (min (tid + pow2 it) nth) dot_v) **
-      pure (c == (pow2 it < nth) /\ SZ.v it < 31)
+  while (let vi = !i; (FStar.SizeT.op_Less_Hat vi size))
+    invariant b.
+      exists* vi vr.
+        gpu ** // infer automatically
+        GA.gpu_pts_to_array_slice a 0 (SZ.v size) v ** // infer automatically
+        Pulse.Lib.Reference.pts_to i vi **
+        Pulse.Lib.Reference.pts_to r vr **
+        pure (b == (vi <^ size))
   {
-    let it = !n <: nat;
-    iteration nth r dot_v tid it;
-    assume_ (pure (SZ.v it < 30)); // FIXME: overflow
-    n := it +^ 1sz;
+    let vi = !i;
+    // FIXME: using #t instead of #tt (t = SizeT.t) gives a terrible error
+    let v = gpu_array_read #tt #(SZ.v size) #0 #(SZ.v size) a #1.0R vi;
+    let vr = !r;
+    let vr' = add vr v;
+    r := vr';
   };
-  
-  (**)let it = !n;
-  (**)FStar.Math.Lemmas.modulo_lemma tid (pow2 it);
-  // assert (pure (pow2 it >= nth /\ tid < nth /\ (div_pow2 it tid) == (tid = 0)));
-
-  // rewrite (if_ (div_pow2 (reveal it) tid) (gpu_pts_to_slice_sum r tid (min (tid + pow2 (reveal it)) nth) dot_v))
-  //     as  (if_ (tid = 0) (gpu_pts_to_slice_sum r tid nth dot_v));
-
-  if (tid = 0sz) {
-    (**)if_elim_true (gpu_pts_to_slice_sum r tid (min (tid + pow2 it) nth) dot_v);
-    (**)if_intro_true (gpu_pts_to_slice_sum r 0 nth dot_v);
-    (**)fold (kpost nth ga1 ga2 r #s1 #s2 tid);
-  } else {
-    (**)fold (kpost nth ga1 ga2 r #s1 #s2 tid);
-  };
+  fold (gpu_pts_to_array a v);
+  !r
 }
 
-let shared_array (#nth : nat { nth <> 0 }) (ga : gpu_array U64.t nth) (#v: Seq.seq U64.t { Seq.length v == nth }) (_: nat): slprop =
-  gpu_pts_to_array ga #(1.0R /. Real.of_int nth) v
-
-ghost
-fn share_array
-  (#nth : nat { nth <> 0 })
-  (ga : gpu_array U64.t nth)
-  (#v: erased (Seq.seq U64.t) { reveal (Seq.length v) == nth })
-  requires gpu_pts_to_array ga #1.0R v
-  ensures  bigstar 0 nth (shared_array #nth ga #v)
+(* Reduces a simple scalar array with the addition operation, leaving
+the result in the 0th index of the original array (overwriting that element). *)
+[@@CPrologue "__global__"]
+fn k_reduce_and_set
+  (#tt : Type0)
+  {| d : simple_scalar tt |}
+  (size : SZ.t)
+  (a : gpu_array tt size)
+  (#v : erased (seq tt))
+  ()
+  requires gpu ** (GA.gpu_pts_to_array a v ** pure (size > 0))
+  ensures  gpu ** (exists* v'. GA.gpu_pts_to_array a v')
 {
-  rewrite gpu_pts_to_array ga #1.0R v
-    as gpu_pts_to_array ga #(1.0R /. of_int 1) v;
-  admit();
+  let r = k_reduce size a;
+  unfold (gpu_pts_to_array a v);
+  gpu_array_write #tt #(SZ.v size) #0 #(SZ.v size) a 0sz r;
+  with v'. assert (gpu_pts_to_array_slice a 0 (SZ.v size) v');
+  fold (gpu_pts_to_array a v');
 }
 
-ghost
-fn gather_array
-  (#nth : nat { nth <> 0 })
-  (ga : gpu_array U64.t nth)
-  (#v: erased (Seq.seq U64.t) { reveal (Seq.length v) == nth })
-  requires bigstar 0 nth (shared_array #nth ga #v)
-  ensures  gpu_pts_to_array ga #1.0R v
+inline_for_extraction noextract
+[@@noextract_to "krml"]	
+fn copy_to_gpu
+  (#t:Type0)
+  {| d : sized t |}
+  (sz : SZ.t)
+  (a : A.array t)
+  (#v : erased (seq t))
+  requires cpu ** A.pts_to a v
+  returns  ga : GA.gpu_array t sz
+  ensures  cpu ** A.pts_to a v ** GA.gpu_pts_to_array ga v
 {
-  admit();
+  let ga = gpu_array_alloc #t #d sz;
+  gpu_memcpy_host_to_device a ga sz;
+  ga
 }
 
-fn main
-  (a1 a2: array U64.t)
-  (v1 v2: erased (Seq.Base.seq U64.t))
-  (#_: squash (Seq.length v1 = size /\ Seq.length v2 = size))
-  requires cpu ** A.pts_to a1 v1 ** A.pts_to a2 v2
-  returns  dp: U64.t
-  ensures  cpu ** A.pts_to a1 v1 ** A.pts_to a2 v2 ** pure (dp == sum_seq (mul v1 v2) 0 size)
+inline_for_extraction noextract
+[@@noextract_to "krml"]	
+fn reduce
+  (#t : Type0)
+  {| d : simple_scalar t |}
+  (a : array t)
+  (size : SZ.t)
+  (#v : erased (seq t))
+  requires cpu
+        ** A.pts_to a v
+        ** pure (size > 0 /\
+                 Seq.length v == size)
+  returns  r : t
+  ensures  cpu ** (exists* v'. A.pts_to a v')
 {
-  let ar = A.alloc #U64.t 0UL size;
-
-  let ga1 = gpu_array_alloc #U64.t size;
-  let ga2 = gpu_array_alloc #U64.t size;
-
-  GPU.Array.gpu_memcpy_host_to_device a1 ga1 size;
-  GPU.Array.gpu_memcpy_host_to_device a2 ga2 size;
-  
-  let gr = gpu_array_alloc #U64.t size;
-
-  // Slicing the arrays
-  (**)share_array ga1;
-  (**)share_array ga2;
-  (**)gpu_array_slice_1_underspec gr;
-
-  // Boring combination of resources
-  (**)bigstar_zip 0 size (shared_array ga1) (shared_array ga2);
-  (**)bigstar_zip 0 size _ (gpu_pts_to_array1 gr);
-  (**)rewrite
-    (bigstar 0 size
-      (fun i -> ((shared_array #size ga1 #v1 i **
-                 shared_array #size ga2 #v2 i) **
-                 gpu_pts_to_array1 gr i)))
-  as
-    (bigstar 0 size (fun i -> kpre size ga1 ga2 gr #v1 #v2 i))
-    by tadmit ();
-  (**)bigstar_uneta ();
-
-  rewrite
-    bigstar 0 size
-      (kpre size ga1 ga2 gr #v1 #v2)
-  as
-    bigstar 0 (1 * SZ.v size)
-      (kpre size ga1 ga2 gr #v1 #v2);
-
-  launch_kernel_n_m_barrier #0 1sz size
-    #(kpre size ga1 ga2 gr #v1 #v2)
-    #(kpost size ga1 ga2 gr #v1 #v2)
-    #(barrier_matrix size gr (mul v1 v2))
-    (fun etid -> kernel size ga1 ga2 gr #v1 #v2 etid);
-
-  (**)bigstar_eta ();
-  // TODO:
-  (**)drop_
-        (bigstar 0 (1 * SZ.v size) (fun i -> kpost size ga1 ga2 gr #v1 #v2 i));
-  (**)assume_
-        (bigstar 0 size
-          (fun i -> ((gpu_pts_to_array #U64.t #size ga1 #(1.0R /. Real.of_int size) v1 **
-                    gpu_pts_to_array #U64.t #size ga2 #(1.0R /. Real.of_int size) v2) **
-                    if_ (op_Equality #int i 0) (gpu_pts_to_slice_sum gr 0 size (mul v1 v2)))
-        ));
-  
-  (**)bigstar_unzip 0 size _ _;
-  (**)bigstar_unzip 0 size _ _;
-  
-  (**)bigstar_uneta () #0 #0 #size #(shared_array #size ga1 #v1);
-  gather_array ga1;
-  (**)bigstar_uneta () #0 #0 #size #(shared_array #size ga2 #v2);
-  gather_array ga2;
-
-  bigstar_if_elim #_ #0 #size 0 (fun _ -> gpu_pts_to_slice_sum #size gr 0 size (mul v1 v2));
-
-  unfold gpu_pts_to_slice_sum;
-  if_elim_true _;
-  unfold gpu_pts_to_slice_sum_inner;
-  with res. assert (gpu_pts_to_array_slice gr 0 size res);
-  fold (gpu_pts_to_array #U64.t #size gr #1.0R res);
-
-  // TODO: don't copy whole array
-  GPU.Array.gpu_memcpy_device_to_host ar gr size;
-
-  gpu_array_free ga1;
-  gpu_array_free ga2;
-  gpu_array_free gr;
-
-  let dp = ar.(0sz);
-  A.free ar;
-  dp
+  let ga = copy_to_gpu size a;
+  launch_kernel_1
+    (k_reduce_and_set #t #d size ga #v);
+  gpu_memcpy_device_to_host a ga size;
+  gpu_array_free ga;
+  with v'. assert (A.pts_to a v');
+  assert (pure (Seq.length v' > 0));
+  let r = Pulse.Lib.Array.op_Array_Access #t a 0sz #1.0R #v';
+  r
 }
+
+module U64 = FStar.UInt64
+module F32 = GPU.Float32
+
+(*
+fn reduce_F32
+  (a : array F32.t)
+  (size : SZ.t)
+  (#v : erased (seq F32.t))
+  requires cpu
+        ** A.pts_to a v
+        ** pure (size > 0 /\
+                 Seq.length v == size)
+  returns  r : F32.t
+  ensures  cpu ** (exists* v'. A.pts_to a v')
+{
+  reduce #F32.t a size
+}
+
