src/examples/GPU.Polymorphism1.fst
@@ -1,0 +1,84 @@
+module GPU.Polymorphism1
+
+(* Testing basic polymorphism *)
+
+#lang-pulse
+
+open Pulse
+open FStar.Mul
+open GPU
+
+inline_for_extraction noextract
+fn kswap
+  (#t : Type0)
+  (r1 r2 : gpu_ref t)
+  (#v1 #v2 : erased t)
+  requires gpu ** (gpu_pts_to r1 v1 ** gpu_pts_to r2 v2)
+  ensures  gpu ** (gpu_pts_to r1 v2 ** gpu_pts_to r2 v1)
+{
+  let v1 = gpu_read r1;
+  let v2 = gpu_read r2;
+  gpu_write r1 v2;
+  gpu_write r2 v1;
+}
+
+inline_for_extraction noextract
+fn swap_via_gpu
+  (#t : Type0)
+  {| sized t |}
+  (r1 r2 : ref t)
+  (#v1 #v2 : erased t)
+  requires cpu ** (pts_to r1 v1 ** pts_to r2 v2)
+  ensures  cpu ** (pts_to r1 v2 ** pts_to r2 v1)
+{
+  let gr1 = gpu_alloc0 #t ();
+  let gr2 = gpu_alloc0 #t ();
+  GPU.Ref.gpu_memcpy_host_to_device r1 gr1;
+  GPU.Ref.gpu_memcpy_host_to_device r2 gr2;
+  launch_kernel_1 (fun () -> kswap gr1 gr2 #v1 #v2);
+  GPU.Ref.gpu_memcpy_device_to_host r1 gr1;
+  GPU.Ref.gpu_memcpy_device_to_host r2 gr2;
+  gpu_free gr1;
+  gpu_free gr2;
+}
+
+module U64 = FStar.UInt64
+module F32 = GPU.Float32
+
+[@@CPrologue "__global__"]
+fn kswap_U64
+  (r1 r2 : gpu_ref U64.t)
+  (#v1 #v2 : erased _)
+  requires gpu ** (gpu_pts_to r1 v1 ** gpu_pts_to r2 v2)
+  ensures  gpu ** (gpu_pts_to r1 v2 ** gpu_pts_to r2 v1)
+{
+  kswap r1 r2 #v1 #v2
+}
+
+[@@CPrologue "__global__"]
+fn kswap_F32
+  (r1 r2 : gpu_ref F32.t)
+  (#v1 #v2 : erased _)
+  requires gpu ** (gpu_pts_to r1 v1 ** gpu_pts_to r2 v2)
+  ensures  gpu ** (gpu_pts_to r1 v2 ** gpu_pts_to r2 v1)
+{
+  kswap r1 r2 #v1 #v2
+}
+(*
+fn swap_U64
+  (r1 r2 : ref U64.t)
+  (#v1 #v2 : erased _)
+  requires cpu ** (pts_to r1 v1 ** pts_to r2 v2)
+  ensures  cpu ** (pts_to r1 v2 ** pts_to r2 v1)
+{
+  swap_via_gpu r1 r2 #v1 #v2
+}
+
+fn swap_F32
+  (r1 r2 : ref F32.t)
+  (#v1 #v2 : erased _)
+  requires cpu ** (pts_to r1 v1 ** pts_to r2 v2)
+  ensures  cpu ** (pts_to r1 v2 ** pts_to r2 v1)
+{
+  swap_via_gpu r1 r2 #v1 #v2
+}
